src/semantic_base_proofs.v
@@ -18,7 +18,7 @@ Fixpoint expr_freefullvars (e : expr) : Ensemble var :=
     | Const _ _ => Empty_set _
     | ExpVar v | Shuffle v _ => Singleton _ v
     | Tuple el | BuildArray el => exprl_freefullvars el
-    | Not e | Shift _ e _ | Bitmask e _ => expr_freefullvars e
+    | Not e | Shift _ e _ | Bitmask e _ | Coercion e _ => expr_freefullvars e
     | Log _ e1 e2 | Arith _ e1 e2 => Union _ (expr_freefullvars e1) (expr_freefullvars e2)
     | Pack e1 e2 _ => Union _ (expr_freefullvars e1) (expr_freefullvars e2)
     | Fun _ exprl | Fun_v _ _ exprl => exprl_freefullvars exprl
@@ -88,6 +88,7 @@ Fixpoint expr_freevars (e : expr) : Ensemble ident :=
     | Shuffle v _ => var_freevars v
     | Bitmask expr aexpr => Union ident (expr_freevars expr) (aexpr_freevars aexpr)
     | Pack e1 e2 _ => Union ident (expr_freevars e1) (expr_freevars e2)
+    | Coercion e _ => expr_freevars e
     | Fun f exprl => Union ident (Singleton ident f) (exprl_freevars exprl)
     | Fun_v f aexpr exprl => Union ident (Singleton ident f) (Union ident (aexpr_freevars aexpr) (exprl_freevars exprl))
     end
@@ -665,7 +666,7 @@ Fixpoint is_subexpr (e' e : expr) : Prop :=
     | Const _ _ | ExpVar _ => False
     | Shuffle v _ => ExpVar v = e'
     | Fun _ el | Fun_v _ _ el | Tuple el | BuildArray el => is_subexpr_l e' el
-    | Not e | Shift _ e _ | Bitmask e _ => is_subexpr e' e
+    | Not e | Shift _ e _ | Bitmask e _ | Coercion e _ => is_subexpr e' e
     | Log _ e1 e2 | Arith _ e1 e2 | Pack e1 e2 _ => is_subexpr e' e1 \/ is_subexpr e' e2
     end
 with is_subexpr_l e' el :=
@@ -687,7 +688,7 @@ Lemma is_subexpr_trans:
         is_subexpr e1 e3.
 Proof.
     move=> e1 e2 e3; move: e3.
-    refine (expr_find _ (fun eL => is_subexpr e1 e2 -> is_subexpr_l e2 eL -> is_subexpr_l e1 eL) _ _ _ _ _ _ _ _ _ _ _ _ _ _ _); simpl.
+    refine (expr_find _ (fun eL => is_subexpr e1 e2 -> is_subexpr_l e2 eL -> is_subexpr_l e1 eL) _ _ _ _ _ _ _ _ _ _ _ _ _ _ _ _); simpl.
     {
         move=> z o is_sub [HEq|[]].
         rewrite HEq in is_sub.
@@ -748,6 +749,10 @@ Proof.
         rewrite HEq in is_sub; simpl in is_sub; trivial.
     }
     {
+        move=> e HRec l is_sub [HEq|is_sub']; auto.
+        rewrite HEq in is_sub; simpl in is_sub; assumption.
+    }
+    {
         move=> _ [].
     }
     {
@@ -762,7 +767,7 @@ Lemma is_subexpr_freefullvars:
 Proof.
     move=> e1 e2 is_sub v HIn; move: e2 is_sub.
     refine (expr_find _ (fun exprl =>
-        is_subexpr_l e1 exprl -> In _ (exprl_freefullvars exprl) v) _ _ _ _ _ _ _ _ _ _ _ _ _ _ _); simpl.
+        is_subexpr_l e1 exprl -> In _ (exprl_freefullvars exprl) v) _ _ _ _ _ _ _ _ _ _ _ _ _ _ _ _); simpl.
     {
         move=> z o [H|[]].
         rewrite H in HIn; simpl in HIn.
@@ -820,6 +825,10 @@ Proof.
     }
     {
         move=> i a el HRec [H|is_sub]; auto.
+        rewrite H in HIn; simpl in HIn; assumption.
+    }
+    {
+        move=> e HRec l [H|is_sub]; auto.
         rewrite H in HIn; simpl in HIn; assumption.
     }
     {
