src/normalization/collect.v
@@ -61,6 +61,7 @@ Function collect_expr (e : expr) : iset.t :=
     | Shuffle v _ => collect_var v
     | Bitmask expr aexpr => iset.union (collect_expr expr) (collect_aexpr aexpr)
     | Pack e1 e2 _ => iset.union (collect_expr e1) (collect_expr e2)
+    | Coercion e _ => collect_expr e
     | Fun f exprl => iset.union (iset.singleton f) (collect_exprl exprl)
     | Fun_v f aexpr exprl => iset.union (iset.singleton f) (iset.union (collect_aexpr aexpr) (collect_exprl exprl))
     end
